Foundation/FirstOrder/Z/Ordinal.lean
@@ -53,7 +53,7 @@ lemma mem_trans {x y z : V} (H : IsTransitive z) (hxy : x ∈ y) (hyz : y ∈ z)
 
 lemma succ {x : V} (h : IsTransitive x) : IsTransitive (succ x) := ⟨by
   intro y hy
-  rcases show y = x ∨ y ∈ x by simpa using hy with (rfl | hy)
+  rcases show y = x ∨ y ∈ x by simpa [mem_succ_iff] using hy with (rfl | hy)
   · simp
   · exact subset_trans (h.transitive y hy) (by simp)⟩
 
@@ -65,6 +65,12 @@ lemma succ {x : V} (h : IsTransitive x) : IsTransitive (succ x) := ⟨by
   case succ =>
     intro x hx ih
     exact ih.succ
+
+lemma union {x y : V} [hx : IsTransitive x] [hy : IsTransitive y] : IsTransitive (x ∪ y) := ⟨by
+  simp only [mem_union_iff]
+  rintro z (hzx | hzy)
+  · exact subset_trans (hx.transitive z hzx) (by simp)
+  · exact subset_trans (hy.transitive z hzy) (by simp)⟩
 
 /-
 @[simp] lemma IsTransitive.ω : IsTransitive (ω : V) := by
@@ -87,7 +93,7 @@ lemma succ {x : V} (h : IsTransitive x) : IsTransitive (succ x) := ⟨by
     simp [zero_def]
   case succ =>
     intro x hx ih z hz
-    rcases show z = x ∨ z ∈ x by simpa using hz with (rfl | hz)
+    rcases show z = x ∨ z ∈ x by simpa [mem_succ_iff] using hz with (rfl | hz)
     · exact hx
     · exact ih z hz⟩
 
@@ -112,7 +118,9 @@ instance IsOrdinal.definable : ℒₛₑₜ-predicate[V] IsOrdinal := IsOrdinal.
 
 namespace IsOrdinal
 
-lemma of_lt {α β : V} (h : IsOrdinal α) (lt : β < α) : IsOrdinal β where
+variable {α β γ : V}
+
+lemma of_mem [h : IsOrdinal α] (lt : β ∈ α) : IsOrdinal β where
   transitive γ hzy δ hvz := by
     have hzx : γ ∈ α := h.transitive _ lt _ hzy
     have hvx : δ ∈ α := h.transitive _ hzx _ hvz
@@ -132,12 +140,12 @@ lemma of_lt {α β : V} (h : IsOrdinal α) (lt : β < α) : IsOrdinal β where
 
 @[simp] protected instance zero : IsOrdinal (0 : V) := .empty
 
-protected instance succ {α : V} [h : IsOrdinal α] : IsOrdinal (succ α) where
+protected instance succ [h : IsOrdinal α] : IsOrdinal (succ α) where
   transitive := h.toIsTransitive.succ.transitive
   trichotomy β₁ h₁ β₂ h₂ := by
-    rcases show β₁ = α ∨ β₁ ∈ α by simpa using h₁ with (rfl | h₁)
-    · rcases show β₂ = β₁ ∨ β₂ ∈ β₁ by simpa using h₂ with (rfl | h₂) <;> simp_all
-    · rcases show β₂ = α ∨ β₂ ∈ α by simpa using h₂ with (rfl | h₂)
+    rcases show β₁ = α ∨ β₁ ∈ α by simpa [mem_succ_iff] using h₁ with (rfl | h₁)
+    · rcases show β₂ = β₁ ∨ β₂ ∈ β₁ by simpa [mem_succ_iff] using h₂ with (rfl | h₂) <;> simp_all
+    · rcases show β₂ = α ∨ β₂ ∈ α by simpa [mem_succ_iff] using h₂ with (rfl | h₂)
       · simp_all
       · exact h.trichotomy β₁ h₁ β₂ h₂
 
@@ -147,8 +155,111 @@ protected instance nat : α ∈ (ω : V) → IsOrdinal (α : V) := by
   case zero => simp [zero_def]
   case succ => intro α hα H; exact H.succ
 
-@[simp] instance ω : IsOrdinal (ω : V) where
-  trichotomy := by sorry
+lemma mem_of_ssubset [hα : IsOrdinal α] [hβ : IsOrdinal β] : α ⊊ β → α ∈ β := by
+  intro ss
+  have : ∃ γ, (γ ∈ β ∧ γ ∉ α) ∧ ∀ δ ∈ β, δ ∉ α → δ ∉ γ := by
+    simpa using foundation (β \ α) (isNonempty_sdiff_of_ssubset ss)
+  rcases this with ⟨γ, ⟨hγβ, hγα⟩, Hγ⟩
+  have Hγα : γ ⊆ α := by
+    intro ξ hξγ
+    have hξβ : ξ ∈ β := hβ.transitive γ hγβ _ hξγ
+    by_contra hξα
+    have : ξ ∉ γ := Hγ ξ hξβ hξα
+    contradiction
+  have Hαγ : α ⊆ γ := by
+    intro ξ hξα
+    have : ξ ∈ β := ss.subset _ hξα
+    have : ξ ∈ γ ∨ (ξ = γ ∨ γ ∈ ξ) := hβ.trichotomy ξ this γ hγβ
+    rcases this with (hξγ | C)
+    · exact hξγ
+    · have : γ ∈ α := by
+        rcases C with (rfl | h)
+        · assumption
+        · exact hα.transitive _ hξα _ h
+      contradiction
+  have : α = γ := subset_antisymm Hαγ Hγα
+  rcases this
+  assumption
+
+@[grind] lemma ssubset_iff [hα : IsOrdinal α] [hβ : IsOrdinal β] : α ⊊ β ↔ α ∈ β :=
+  ⟨mem_of_ssubset, fun hαβ ↦ ⟨hβ.transitive _ hαβ, ne_of_mem hαβ⟩⟩
+
+@[grind] lemma subset_iff [hα : IsOrdinal α] [hβ : IsOrdinal β] : α ⊆ β ↔ α = β ∨ α ∈ β := by
+  constructor
+  · intro ss
+    by_cases eq : α = β
+    · simp_all
+    · right; exact mem_of_ssubset ⟨ss, eq⟩
+  · rintro (rfl | h)
+    · simp
+    · exact hβ.transitive α h
+
+variable (α β)
+
+lemma subset_or_supset [hα : IsOrdinal α] [hβ : IsOrdinal β] : α ⊆ β ∨ β ⊆ α := by
+  by_contra Aαβ
+  push_neg at Aαβ
+  let C : V := {α' ∈ succ α ; ∃ β, IsOrdinal β ∧ ¬α' ⊆ β ∧ ¬β ⊆ α'}
+  have hαC : α ∈ C := by
+    simp only [mem_sep_iff, mem_succ_iff, mem_irrefl, or_false, true_and, C]
+    exact ⟨β, hβ, Aαβ⟩
+  have : ∃ α₀, (α₀ ∈ succ α ∧ ∃ β, IsOrdinal β ∧ ¬α₀ ⊆ β ∧ ¬β ⊆ α₀) ∧ ∀ γ ∈ C, γ ∉ α₀ := by
+    simpa [C] using foundation C ⟨α, hαC⟩
+  rcases this with ⟨α₀, ⟨hα₀sα, β₀, ordβ₀, Hα₀β₀⟩, Hα₀⟩
+  have ordα₀ : IsOrdinal α₀ := by
+    rcases mem_succ_iff.mp hα₀sα with (rfl | hα₀α)
+    · assumption
+    · exact hα.of_mem hα₀α
+  let γ₀ := α₀ ∪ β₀
+  have : IsOrdinal γ₀ := isOrdinal_iff.mpr ⟨IsTransitive.union, by
+    intro ξ hξγ₀ ζ hζγ₀
+    rcases show ξ ∈ α₀ ∨ ξ ∈ β₀ by simpa [γ₀] using hξγ₀ with (hξα₀ | hξβ₀)
+    · have : IsOrdinal ξ := of_mem hξα₀
+      rcases show ζ ∈ α₀ ∨ ζ ∈ β₀ by simpa [γ₀] using hζγ₀ with (hζα₀ | hζβ₀)
+      · exact ordα₀.trichotomy ξ hξα₀ ζ hζα₀
+      · have : IsOrdinal ζ := of_mem hζβ₀
+        have : ξ ⊆ ζ ∨ ζ ⊆ ξ := by
+          by_contra A; push_neg at A
+          have : ξ ∈ C := mem_sep_iff.mpr ⟨hα.succ.transitive α₀ hα₀sα ξ hξα₀, ζ, of_mem hζβ₀, A⟩
+          exact Hα₀ ξ this hξα₀
+        grind
+    · have : IsOrdinal ξ := of_mem hξβ₀
+      rcases show ζ ∈ α₀ ∨ ζ ∈ β₀ by simpa [γ₀] using hζγ₀ with (hζα₀ | hζβ₀)
+      · have : IsOrdinal ζ := of_mem hζα₀
+        have : ξ ⊆ ζ ∨ ζ ⊆ ξ := by
+          by_contra A; push_neg at A
+          have : ζ ∈ C := mem_sep_iff.mpr ⟨hα.succ.transitive α₀ hα₀sα ζ hζα₀, ξ, inferInstance, by grind⟩
+          exact Hα₀ _ this hζα₀
+        grind
+      · have : ζ ∈ ξ ∨ ζ = ξ ∨ ξ ∈ ζ := ordβ₀.trichotomy ζ hζβ₀ ξ hξβ₀
+        grind⟩
+  have : γ₀ = α₀ ∨ γ₀ = β₀ := by
+    by_contra A; push_neg at A
+    have : α₀ ∈ γ₀ := ssubset_iff.mp ⟨by simp [γ₀], by grind⟩
+    have hα₀β₀ : α₀ ∈ β₀ := by simpa [γ₀] using this
+    have : β₀ ∈ γ₀ := ssubset_iff.mp ⟨by simp [γ₀], by grind⟩
+    have hβ₀α₀ : β₀ ∈ α₀ := by simpa [γ₀] using this
+    exact mem_asymm hα₀β₀ hβ₀α₀
+  rcases this with (e | e)
+  · have : β₀ ⊆ α₀ := by simpa [γ₀] using e
+    grind
+  · have : α₀ ⊆ β₀ := by simpa [γ₀] using e
+    grind
+
+lemma mem_trichotomy [hα : IsOrdinal α] [hβ : IsOrdinal β] : α ∈ β ∨ α = β ∨ β ∈ α := by
+  have : α ⊆ β ∨ β ⊆ α := subset_or_supset α β
+  grind
+
+variable {α β}
+
+lemma of_transitive_of_isOrdinal (tr : IsTransitive α) (H : ∀ β ∈ α, IsOrdinal β) : IsOrdinal α where
+  trichotomy ξ hξα ζ hζα :=
+    have : IsOrdinal ξ := H ξ hξα
+    have : IsOrdinal ζ := H ζ hζα
+    mem_trichotomy ξ ζ
+
+@[simp] instance ω : IsOrdinal (ω : V) :=
+  of_transitive_of_isOrdinal inferInstance fun _ hn ↦ IsOrdinal.nat hn
 
 end IsOrdinal
 
